arrays and array pointers

ulib/experimental/Steel.Array.fst
@@ -1,5 +1,5 @@
 (*
-   Copyright 2020 Microsoft Research
+   Copyright 2021 Microsoft Research
 
    Licensed under the Apache License, Version 2.0 (the "License");
    you may not use this file except in compliance with the License.
@@ -15,27 +15,824 @@
 *)
 
 module Steel.Array
-
 open Steel.Effect.Atomic
 open Steel.Reference
 
-let array t = ref (Seq.seq t)
+let seq_facts () : Lemma (
+  (forall (t: Type) (s: Seq.seq t) .
+    Seq.length s == 0 ==> s == Seq.empty) /\
+  (forall (t: Type) (a: t) (s: Seq.seq t) .
+    Seq.head (Seq.cons a s) == a /\ Seq.tail (Seq.cons a s) == s) /\
+  (forall (t: Type) (s: Seq.seq t) .
+    Seq.length s > 0 ==>
+    s == Seq.cons (Seq.head s) (Seq.tail s))
+) =
+  let e
+    (t: Type) (s: Seq.seq t)
+  : Lemma
+    (Seq.length s == 0 ==> s == Seq.empty)
+  =
+    if Seq.length s = 0 then assert (s `Seq.equal` Seq.empty)
+  in
+  let f
+    (t: Type) (a: t) (s: Seq.seq t)
+  : Lemma
+    (Seq.head (Seq.cons a s) == a /\ Seq.tail (Seq.cons a s) == s)
+  = Seq.head_cons a s;
+    Seq.lemma_tl a s
+  in
+  let g
+    (t: Type) (s: Seq.seq t)
+  : Lemma
+    (Seq.length s > 0 ==> s == Seq.cons (Seq.head s) (Seq.tail s))
+  =
+    if Seq.length s > 0
+    then Seq.cons_head_tail s
+  in
+  Classical.forall_intro_2 e;
+  Classical.forall_intro_3 f;
+  Classical.forall_intro_2 g
 
-let is_array r = ptr r
-let array_sel r = ptr_sel r
+let fits32 (x: nat) : Tot prop = FStar.UInt.fits x U32.n == true
+let array1 (t: Type) : Tot Type = (x: Seq.seq (ref t) {fits32 (Seq.length x)})
+let array2 (t: Type) : Tot Type = Ghost.erased (array1 t)
+noeq
+type array t = {
+  base: array1 t;
+  from: U32.t;
+  to: (to: Ghost.erased U32.t { U32.v from <= U32.v to /\ U32.v to <= Seq.length base })
+}
+let len #t a = a.to `U32.sub` a.from
 
-let alloc x n =
-  let s = Seq.create (U32.v n) x in
-  alloc s
+let vnil_rewrite
+  (t: Type)
+  (x: t_of emp)
+: GTot (Seq.lseq t 0)
+= Seq.empty
 
-let index r i =
-  let h = get() in
-  let s = read r in
-  Seq.index s (U32.v i)
+let vnil
+  (t: Type)
+: Pure vprop
+  (requires True)
+  (ensures (fun v -> t_of v == Seq.lseq t 0))
+= vrewrite emp (vnil_rewrite t)
 
-let upd r i x =
-  let s = read r in
-  let s' = Seq.upd s (U32.v i) x in
-  write r s'
+let vcons_rewrite
+  (#t: Type)
+  (n: Ghost.erased nat)
+  (r: Ghost.erased (ref t))
+  (v: vprop)
+  (sq: squash (t_of v == Seq.lseq t n))
+  (xy: t_of (vptr r `star` v))
+: GTot (Seq.lseq t (n + 1))
+= Seq.cons (fst xy) (snd xy)
 
-let free r = free r
+let vcons
+  (#t: Type)
+  (n: Ghost.erased nat)
+  (r: Ghost.erased (ref t))
+  (v: vprop)
+: Pure vprop
+  (requires (t_of v == Seq.lseq t n))
+  (ensures (fun v' -> t_of v' == Seq.lseq t (n + 1)))
+= vrewrite (vptr r `star` v) (vcons_rewrite n r v ())
+
+let rec varray1
+  (#t: Type0)
+  (a: array2 t)
+: Pure vprop
+  (requires True)
+  (ensures (fun v -> t_of v == Seq.lseq t (Seq.length a)))
+  (decreases (Seq.length a))
+= if Seq.length a = 0
+  then vnil t
+  else vcons (Seq.length a - 1) (Seq.index a 0) (varray1 (Seq.slice a 1 (Seq.length a)))
+
+[@@ __steel_reduce__]
+unfold
+let sel_varray1 (#a:Type) (#p:vprop) (r:array2 a)
+  (h:rmem p{FStar.Tactics.with_tactic selector_tactic (can_be_split p (varray1 r) /\ True)})
+: GTot (Seq.lseq a (Seq.length r))
+= let x : t_of (varray1 r) = h (varray1 r) in
+  x
+
+let sel_varray2
+  (#a: Type0)
+  (r: array2 a)
+: Tot (selector (Seq.lseq a (Seq.length r)) (hp_of (varray1 r)))
+= fun h -> sel_of (varray1 r) h
+
+[@@ __steel_reduce__]
+let varray2' (#a: Type0) (r: array2 a) : vprop' =
+  {hp = hp_of (varray1 r);
+   t = Seq.lseq a (Seq.length r);
+   sel = sel_varray2 r}
+
+[@@ __steel_reduce__]
+let varray2 r = VUnit (varray2' r)
+
+let varray9
+  (#t: Type0)
+  (a: array t)
+: Tot vprop
+= varray2 (Seq.slice a.base (U32.v a.from) (U32.v a.to))
+
+let is_array #a r = hp_of (varray9 r)
+
+let array_sel #a r = fun h -> sel_of (varray9 r) h
+
+let intro_varray
+  (#opened: _)
+  (#t: Type)
+  (q: array2 t)
+  (r: array t)
+: SteelGhost unit opened
+    (varray2 q)
+    (fun _ -> varray r)
+    (fun _ -> Ghost.reveal q `Seq.equal` Seq.slice r.base (U32.v r.from) (U32.v r.to))
+    (fun h _ h' ->
+      (h (varray2 q) <: Seq.seq t) == h' (varray r)
+    )
+=
+  change_slprop_rel
+    (varray2 q)
+    (varray r)
+    (fun (x: t_of (varray2 q)) (y: t_of (varray r)) -> (x <: Seq.seq t) == y)
+    (fun _ -> ())
+
+let elim_varray
+  (#opened: _)
+  (#t: Type)
+  (r: array t)
+: SteelGhost (array2 t) opened
+    (varray r)
+    (fun q -> varray2 q)
+    (fun _ -> True)
+    (fun h q h' ->
+      Ghost.reveal q == Seq.slice r.base (U32.v r.from) (U32.v r.to) /\
+      (h (varray r) <: Seq.seq t) == h' (varray2 q)
+    )
+=
+  let q : array2 t = (Seq.slice r.base (U32.v r.from) (U32.v r.to)) in
+  change_slprop_rel
+    (varray r)
+    (varray2 q)
+    (fun (y: t_of (varray r)) (x: t_of (varray2 q)) -> (x <: Seq.seq t) == y)
+    (fun _ -> ());
+  q
+
+let intro_varray2
+  (#opened: _)
+  (#t: Type)
+  (q: array2 t)
+: SteelGhost unit opened
+    (varray1 q)
+    (fun _ -> varray2 q)
+    (fun _ -> True)
+    (fun h _ h' ->
+      (h' (varray2 q) <: Seq.seq t) == sel_varray1 q h 
+    )
+=
+  change_slprop_rel
+    (varray1 q)
+    (varray2 q)
+    (fun (x: t_of (varray1 q)) (y: t_of (varray2 q)) -> (x <: Seq.seq t) == y)
+    (fun _ -> ())
+
+let elim_varray2
+  (#opened: _)
+  (#t: Type)
+  (r: array2 t)
+: SteelGhost unit opened
+    (varray2 r)
+    (fun _ -> varray1 r)
+    (fun _ -> True)
+    (fun h _ h' ->
+      (h (varray2 r) <: Seq.seq t) == sel_varray1 r h'
+    )
+=
+  change_slprop_rel
+    (varray2 r)
+    (varray1 r)
+    (fun (y: t_of (varray2 r)) (x: t_of (varray1 r)) -> (x <: Seq.seq t) == y)
+    (fun _ -> ())
+
+let intro_vnil1
+  (#opened: _)
+  (t: Type)
+: SteelGhost (array2 t) opened
+    emp
+    (fun r -> varray1 r)
+    (fun _ -> True)
+    (fun _ r _ -> Seq.length r == 0)
+=
+  intro_vrewrite emp (vnil_rewrite t);
+  let r : array2 t = Seq.empty in
+  change_slprop
+    (vrewrite emp (vnil_rewrite t))
+    (varray1 r)
+    (Ghost.hide (Seq.empty #t <: t_of (vrewrite emp (vnil_rewrite t))))
+    (Ghost.hide (Seq.empty #t <: t_of (varray1 r)))
+    (fun _ -> ());
+  r
+
+let intro_vnil
+  (#opened: _)
+  (t: Type)
+: SteelGhost (array2 t) opened
+    emp
+    (fun r -> varray2 r)
+    (fun _ -> True)
+    (fun _ r h' ->
+      Ghost.reveal r == Seq.empty /\
+      h' (varray2 r) == Seq.empty
+    )
+=
+  seq_facts ();
+  let res = intro_vnil1 t in
+  intro_varray2 res;
+  res
+
+let intro_vcons1
+  (#opened: _)
+  (#t: Type)
+  (r: Ghost.erased (ref t))
+  (a: array2 t)
+: SteelGhost (array2 t) opened
+    (vptr r `star` varray1 a)
+    (fun a' -> varray1 a')
+    (fun _ -> fits32 (Seq.length a + 1))
+    (fun h a' h' ->
+      Ghost.reveal a' == Seq.cons (Ghost.reveal r) a /\
+      (sel_varray1 a' h' <: Seq.seq t) ==
+        Seq.cons (h (vptr r)) (sel_varray1 a h)
+    )
+=
+  seq_facts ();
+  reveal_star (vptr r) (varray1 a); // FIXME: WHY WHY WHY?
+  intro_vrewrite (vptr r `star` varray1 a) (vcons_rewrite (Seq.length a) r (varray1 a) ());
+  let a' : array2 t = Seq.cons (Ghost.reveal r) a in
+  change_equal_slprop
+    (vrewrite (vptr r `star` varray1 a) (vcons_rewrite (Seq.length a) r (varray1 a) ()))
+    (varray1 a');
+  a'
+
+let intro_vcons
+  (#opened: _)
+  (#t: Type)
+  (r: Ghost.erased (ref t))
+  (a: array2 t)
+: SteelGhost (array2 t) opened
+    (vptr r `star` varray2 a)
+    (fun a' -> varray2 a')
+    (fun _ -> fits32 (Seq.length a + 1))
+    (fun h a' h' ->
+      Ghost.reveal a' == Seq.cons (Ghost.reveal r) a /\
+      h' (varray2 a') ==
+        Seq.cons (h (vptr r)) (h (varray2 a))
+    )
+= elim_varray2 a;
+  let res = intro_vcons1 r a in
+  intro_varray2 res;
+  res
+
+#set-options "--ide_id_info_off" 
+
+#push-options "--z3rlimit 16"
+#restart-solver
+
+let elim_vcons1
+  (#opened: _)
+  (#t: Type)
+  (a: array2 t)
+: SteelGhost (Ghost.erased (ref t) & array2 t) opened
+    (varray1 a)
+    (fun res -> vptr (pfst res) `star` varray1 (psnd res))
+    (fun _ -> Seq.length a > 0)
+    (fun h res h' ->
+      Seq.length a > 0 /\
+      begin let s = sel_varray1 a h in
+      h' (vptr (pfst res)) == Seq.head s /\
+      Seq.tail s == sel_varray1 (psnd res) h' /\
+      Ghost.reveal a == Seq.cons (Ghost.reveal (pfst res)) (psnd res)
+      end
+    )
+=
+  seq_facts ();
+  let a0 : Ghost.erased (Seq.seq (ref t)) = Ghost.hide (Ghost.reveal a) in // same here
+  let r : Ghost.erased (ref t) = (Seq.head a0) in
+  let q : array2 t = Seq.tail a0 in
+  change_equal_slprop
+    (varray1 a)
+    (vrewrite (vptr (r) `star` varray1 (q)) (vcons_rewrite (Seq.length (q)) (r) (varray1 (q)) ()));
+  elim_vrewrite (vptr (r) `star` varray1 (q)) (vcons_rewrite (Seq.length (q)) (r) (varray1 (q)) ());
+  reveal_star (vptr (r)) (varray1 (q));
+  let res : (Ghost.erased (ref t) & array2 t) = (r, q) in
+  change_equal_slprop
+    (vptr (r) `star` varray1 (q))
+    (vptr (pfst res) `star` varray1 (psnd res));
+  reveal_star (vptr (pfst res)) (varray1 (psnd res));
+  res
+
+#pop-options
+
+let elim_vcons
+  (#opened: _)
+  (#t: Type)
+  (a: array2 t)
+: SteelGhost (Ghost.erased (ref t) & array2 t) opened
+    (varray2 a)
+    (fun res -> vptr (pfst res) `star` varray2 (psnd res))
+    (fun _ -> Seq.length a > 0)
+    (fun h res h' ->
+      Seq.length a > 0 /\
+      begin let s = h (varray2 a) in
+      s == Seq.cons (h' (vptr (pfst res))) (h' (varray2 (psnd res))) /\
+      Ghost.reveal a == Seq.cons (Ghost.reveal (pfst res)) (psnd res)
+      end
+    )
+=
+  elim_varray2 a;
+  let res = elim_vcons1 a in
+  intro_varray2 (psnd res);
+  res
+
+let elim_nil
+  (#opened: _)
+  (#t: Type)
+  (a: array2 t)
+: SteelGhost unit opened
+    (varray2 a)
+    (fun _ -> emp)
+    (fun _ -> Seq.length a == 0)
+    (fun _ _ _ -> True)
+=
+  elim_varray2 a; 
+  change_equal_slprop
+    (varray1 a)
+    (vrewrite emp (vnil_rewrite t));
+  elim_vrewrite emp (vnil_rewrite t)
+
+let seq_append_nil
+  (#t: Type)
+  (a2: Seq.seq t)
+: Lemma
+  (Seq.append Seq.empty a2 == a2)
+  [SMTPat (Seq.append Seq.empty a2)]
+= assert (Seq.append Seq.empty a2 `Seq.equal` a2)
+
+#push-options "--z3rlimit 16"
+#restart-solver
+
+let seq_append_cons
+  (#t: Type)
+  (c: t)
+  (a1 a2: Seq.seq t)
+: Lemma
+  (Seq.append (Seq.cons c a1) a2 == Seq.cons c (Seq.append a1 a2))
+  [SMTPat (Seq.append (Seq.cons c a1) a2)]
+=
+  assert (Seq.append (Seq.cons c a1) a2 `Seq.equal` Seq.cons c (Seq.append a1 a2))
+
+#pop-options
+
+#push-options "--z3rlimit 64"
+#restart-solver
+
+let rec vappend
+  (#opened: _)
+  (#t: Type)
+  (a1 a2: array2 t)
+: SteelGhost (array2 t) opened
+    (varray2 a1 `star` varray2 a2)
+    (fun r -> varray2 r)
+    (fun _ -> fits32 (Seq.length a1 + Seq.length a2))
+    (fun h r h' ->
+      h' (varray2 r) == Seq.append (h (varray2 a1)) (h (varray2 a2)) /\
+      Ghost.reveal r == Seq.append a1 a2
+    )
+    (decreases (Seq.length a1))
+=
+  seq_facts ();
+  if Seq.length a1 = 0
+  then begin
+    elim_nil a1;
+    a2
+  end else begin
+    let hd_tl = elim_vcons a1 in
+    reveal_star_3 (vptr (pfst hd_tl)) (varray2 (psnd hd_tl)) (varray2 a2); // FIXME: WHY WHY WHY?
+    let tl' = vappend (psnd hd_tl) a2 in
+    let res = intro_vcons (pfst hd_tl) tl' in
+    res
+  end
+
+#pop-options
+
+let slice_cons_left
+  (#t: Type)
+  (a: t)
+  (x: Seq.seq t)
+  (i: nat)
+: Lemma
+  ((i > 0 /\ i <= Seq.length x + 1) ==> Seq.slice (Seq.cons a x) 0 i == Seq.cons a (Seq.slice x 0 (i - 1)))
+= if i > 0 && i <= Seq.length x + 1 then assert (Seq.slice (Seq.cons a x) 0 i `Seq.equal` Seq.cons a (Seq.slice x 0 (i - 1)))
+
+let slice_cons_right
+  (#t: Type)
+  (a: t)
+  (x: Seq.seq t)
+  (i: nat)
+: Lemma
+  ((i > 0 /\ i <= Seq.length x + 1) ==> Seq.slice (Seq.cons a x) i (Seq.length x + 1) == Seq.slice x (i - 1) (Seq.length x))
+= if i > 0 && i <= Seq.length x + 1 then assert (Seq.slice (Seq.cons a x) i (Seq.length x + 1) `Seq.equal` Seq.slice x (i - 1) (Seq.length x))
+
+#push-options "--z3rlimit 16"  // 256 --fuel 6 --ifuel 6"
+#restart-solver
+
+let rec vsplit
+  (#opened: _)
+  (#t: Type)
+  (a: array2 t)
+  (i: U32.t)
+: SteelGhost (array2 t & array2 t) opened
+    (varray2 a)
+    (fun res -> varray2 (pfst res) `star` varray2 (psnd res))
+    (fun _ -> U32.v i <= Seq.length a)
+    (fun h res h' ->
+      let s = h (varray2 a) in
+      U32.v i <= Seq.length a /\
+      pfst res `Seq.equal` Seq.slice a 0 (U32.v i) /\
+      psnd res `Seq.equal` Seq.slice a (U32.v i) (Seq.length a) /\
+      h' (varray2 (pfst res)) == Seq.slice s 0 (U32.v i) /\
+      h' (varray2 (psnd res)) `Seq.equal` Seq.slice s (U32.v i) (Seq.length a)
+    )
+    (decreases (U32.v i))
+=
+  seq_facts ();
+  let g0 = gget (varray2 a) in
+  if i = 0ul
+  then begin
+    let n = intro_vnil t in
+    reveal_star (varray2 n) (varray2 a);
+    let res = (n, a) in
+    change_equal_slprop
+      (varray2 n `star` varray2 a)
+      (varray2 (pfst res) `star` varray2 (psnd res));
+    reveal_star (varray2 (pfst res)) (varray2 (psnd res));
+    res
+  end else begin
+    let hd_tl : (Ghost.erased (ref t) & array2 t) = elim_vcons a in
+    reveal_star (vptr (pfst hd_tl)) (varray2 (psnd hd_tl));
+    let j = i `U32.sub` 1ul in
+    assert (U32.v j == U32.v i - 1);
+    let g2_hd = gget (vptr (pfst hd_tl)) in
+    let g2_tl = gget (varray2 (psnd hd_tl)) in
+    slice_cons_left (Ghost.reveal g2_hd) (Ghost.reveal g2_tl) (U32.v i);
+    slice_cons_right (Ghost.reveal g2_hd) (Ghost.reveal g2_tl) (U32.v i);
+    let sl_sr = vsplit (psnd hd_tl) j in
+    reveal_star_3 (vptr (pfst hd_tl)) (varray2 (pfst sl_sr)) (varray2 (psnd sl_sr)); // FIXME: WHY WHY WHY?
+    let sl = intro_vcons (pfst hd_tl) (pfst sl_sr) in
+    reveal_star (varray2 sl) (varray2 (psnd sl_sr));
+    let res = (sl, psnd sl_sr) in
+    change_equal_slprop
+      (varray2 sl `star` varray2 (psnd sl_sr))
+      (varray2 (pfst res) `star` varray2 (psnd res));
+    reveal_star (varray2 (pfst res)) (varray2 (psnd res));
+    res
+  end
+
+#pop-options
+
+[@@erasable]
+noeq
+type ith_t
+  (t: Type)
+= {
+  ith_lhs: array2 t;
+  ith_item: Ghost.erased (ref t);
+  ith_rhs: array2 t;
+}
+
+#push-options "--z3rlimit 16"
+
+let unpack_ith
+  (#opened: _)
+  (#t: Type)
+  (a: array2 t)
+  (i: U32.t)
+: SteelGhost (ith_t t) opened
+    (varray2 a)
+    (fun res -> varray2 res.ith_lhs `star` vptr res.ith_item `star` varray2 res.ith_rhs)
+    (fun _ -> U32.v i < Seq.length a)
+    (fun h res h' ->
+      U32.v i < Seq.length a /\
+      Ghost.reveal a == Seq.append res.ith_lhs (Seq.cons (Ghost.reveal res.ith_item) res.ith_rhs) /\
+      can_be_split (varray2 res.ith_lhs `star` vptr res.ith_item `star` varray2 res.ith_rhs) (varray2 res.ith_lhs) /\
+      can_be_split (varray2 res.ith_lhs `star` vptr res.ith_item `star` varray2 res.ith_rhs) (vptr res.ith_item) /\
+      can_be_split (varray2 res.ith_lhs `star` vptr res.ith_item `star` varray2 res.ith_rhs) (varray2 res.ith_lhs) /\
+      h (varray2 a) == Seq.append (h' (varray2 res.ith_lhs)) (Seq.cons (h' (vptr res.ith_item)) (h' (varray2 res.ith_rhs))) /\
+      Seq.length res.ith_lhs == U32.v i
+    )
+=
+  let m = get #(varray2 a) () in
+  Seq.lemma_split a (U32.v i);
+  Seq.lemma_split (Ghost.reveal m (varray2 a)) (U32.v i);
+  let rsplit = vsplit a i in
+  reveal_star (varray2 (pfst rsplit)) (varray2 (psnd rsplit));
+  let rcons = elim_vcons (psnd rsplit) in
+  reveal_star_3 (varray2 (pfst rsplit)) (vptr (pfst rcons)) (varray2 (psnd rcons));
+  let res = { ith_lhs = pfst rsplit; ith_item = pfst rcons; ith_rhs = psnd rcons } in
+  change_equal_slprop
+    (varray2 (pfst rsplit) `star` vptr (pfst rcons) `star` varray2 (psnd rcons))
+    (varray2 res.ith_lhs `star` vptr res.ith_item `star` varray2 res.ith_rhs);
+  reveal_star_3 (varray2 res.ith_lhs) (vptr res.ith_item) (varray2 res.ith_rhs);
+  res
+
+#pop-options
+
+let pack_ith
+  (#opened: _)
+  (#t: Type)
+  (res: ith_t t)
+  (a: array2 t)
+: SteelGhost unit opened
+    (varray2 res.ith_lhs `star` vptr res.ith_item `star` varray2 res.ith_rhs)
+    (fun _ -> varray2 a)
+    (fun _ ->
+      Ghost.reveal a == Seq.append res.ith_lhs (Seq.cons (Ghost.reveal res.ith_item) res.ith_rhs)
+    )
+    (fun h _ h' ->
+      let i = Seq.length res.ith_lhs in
+      can_be_split (varray2 res.ith_lhs `star` vptr res.ith_item `star` varray2 res.ith_rhs) (varray2 res.ith_lhs) /\
+      can_be_split (varray2 res.ith_lhs `star` vptr res.ith_item `star` varray2 res.ith_rhs) (vptr res.ith_item) /\
+      h' (varray2 a) == Seq.append (h (varray2 res.ith_lhs)) (Seq.cons (h (vptr res.ith_item)) (h (varray2 res.ith_rhs)))
+    )
+=
+  reveal_star_3 (varray2 res.ith_lhs) (vptr res.ith_item) (varray2 res.ith_rhs);
+  let rhs = intro_vcons res.ith_item res.ith_rhs in
+  reveal_star (varray2 res.ith_lhs) (varray2 rhs);
+  let a' = vappend res.ith_lhs rhs in
+  change_equal_slprop (varray2 a') (varray2 a)
+
+let seq_index_append_cons
+  (#t: Type)
+  (i: nat)
+  (a: Seq.seq t) (x: t) (b: Seq.seq t)
+: Lemma
+  (requires (Seq.length a == i))
+  (ensures (Seq.index (Seq.append a (Seq.cons x b)) i == x))
+= ()
+
+let seq_upd_append_cons
+  (#t: Type)
+  (i: nat)
+  (y: t)
+  (a: Seq.seq t) (x: t) (b: Seq.seq t)
+: Lemma
+  (Seq.length a == i ==> Seq.upd (Seq.append a (Seq.cons x b)) i y == Seq.append a (Seq.cons y b))
+=
+  assert (Seq.length a == i ==> Seq.upd (Seq.append a (Seq.cons x b)) i y `Seq.equal` Seq.append a (Seq.cons y b))
+
+let decr32 (a:U32.t) (sq: squash (a <> 0ul)) : Pure U32.t
+  (requires True)
+  (ensures (fun c -> U32.v a - 1 == U32.v c))
+= U32.sub a 1ul
+
+let rec valloc
+  (#t: Type)
+  (i: U32.t)
+  (x: t)
+: Steel (array1 t)
+    emp
+    (fun res -> varray2 res)
+    (fun _ -> True)
+    (fun _ res h' ->
+      Seq.length res == U32.v i /\
+      h' (varray2 res) == Seq.create (U32.v i) x
+    )
+    (decreases (U32.v i))
+=
+  if i = 0ul
+  then
+    let res = intro_vnil t in
+    assert (Seq.create 0 x `Seq.equal` Seq.empty);
+    let res2 : array1 t = Seq.empty in
+    change_equal_slprop
+      (varray2 res)
+      (varray2 res2);
+    return res2
+  else begin
+    let sq : squash (i <> 0ul) = () in
+    let hd = Steel.Reference.alloc x in
+    let j = decr32 i sq in
+    assert (Seq.cons x (Seq.create (U32.v j) x) `Seq.equal` Seq.create (U32.v i) x);
+    let tl = valloc j x in
+    change_equal_slprop
+      (vptr hd)
+      (vptr (Ghost.reveal (Ghost.hide hd)));
+    let res = intro_vcons (Ghost.hide hd) tl in
+    let res2 = Seq.cons hd tl in
+    change_equal_slprop
+      (varray2 res)
+      (varray2 res2);
+    return res2
+  end
+
+let adjacent #_ a b = a.base == b.base /\ Ghost.reveal a.to == b.from
+
+let tmerge
+  (#t: Type)
+  (r1 r2: array t)
+: Pure (array t)
+  (requires (adjacent r1 r2))
+  (ensures (fun r -> length r == length r1 + length r2))
+= {
+  base = r1.base;
+  from = r1.from;
+  to = r2.to;
+}
+
+let merge #t r1 r2 = tmerge r1 r2
+
+let merge_assoc r1 r2 r3 = ()
+
+let tsplit
+  (#t: Type)
+  (r: array t)
+  (i: U32.t)
+: Pure (array t & array t)
+  (requires (U32.v i <= length r))
+  (ensures (fun (rl, rr) ->
+    merge_into rl rr r /\
+    length rl == U32.v i
+  ))
+=
+  let mid = r.from `U32.add` i in
+  let r1 = {
+    base = r.base;
+    from = r.from;
+    to = mid;
+  } in
+  let r2 = {
+    base = r.base;
+    from = mid;
+    to = r.to
+  } in
+  (r1, r2)
+
+let merge_zero_left #t r1 r2 = ()
+
+let merge_zero_right #t r1 r2 = ()
+
+let gsplit #t r i = tsplit r i
+
+let gsplit_unique #t r rl rr = ()
+
+val gsplit0 (#opened: _) (#t:Type) (a:array t) (i:U32.t)
+  : SteelGhost (Ghost.erased (array t & array t)) opened
+          (varray a)
+          (fun res -> varray (pfst res) `star` varray (psnd res))
+          (fun _ -> U32.v i <= length a)
+          (fun h res h' ->
+            let s = h (varray a) in
+            let sl = h' (varray (pfst res)) in
+            let sr = h' (varray (psnd res)) in
+            U32.v i <= length a /\
+            Ghost.reveal res == gsplit a i /\
+            sl == Seq.slice s 0 (U32.v i) /\
+            sr == Seq.slice s (U32.v i) (length a)
+          )
+
+#push-options "--z3rlimit 16"
+let gsplit0 #t a i =
+  let a2 = elim_varray a in
+  Seq.lemma_split a2 (U32.v i);
+  let res2 = vsplit a2 i in
+  let res = tsplit a i in
+  intro_varray (pfst res2) (pfst res);
+  intro_varray (psnd res2) (psnd res);
+  let gres = Ghost.hide res in
+  change_equal_slprop
+    (varray (pfst res))
+    (varray (pfst gres));
+  change_equal_slprop
+    (varray (psnd res))
+    (varray (psnd gres));
+  gres
+#pop-options
+
+let split #t a i =
+  let gres = gsplit0 a i in
+  let res = tsplit a i in
+  change_equal_slprop
+    (varray (pfst gres))
+    (varray (pfst res));
+  change_equal_slprop
+    (varray (psnd gres))
+    (varray (psnd res));
+  return res
+
+val gjoin (#opened: _) (#t:Type) (al ar:array t)
+  : SteelGhost (Ghost.erased (array t)) opened
+          (varray al `star` varray ar)
+          (fun a -> varray a)
+          (fun _ -> adjacent al ar)
+          (fun h a h' ->
+            let s = h' (varray a) in
+            s == (h (varray al) `Seq.append` h (varray ar)) /\
+            merge_into al ar a
+          )
+
+#push-options "--z3rlimit 16"
+let gjoin #t al ar =
+  let al2 = elim_varray al in
+  let ar2 = elim_varray ar in
+  let a2 = vappend al2 ar2 in
+  let a = tmerge al ar in
+  intro_varray a2 a;
+  let res = Ghost.hide a in
+  change_equal_slprop
+    (varray a)
+    (varray (Ghost.reveal res));
+  res
+#pop-options
+
+let join #t al ar =
+  let ga : Ghost.erased (array t) = gjoin al ar in
+  let a = tmerge al ar in
+  change_equal_slprop
+    (varray (Ghost.reveal ga))
+    (varray a);
+  return a
+
+let freeable #t a = a.from == 0ul /\ U32.v a.to == Seq.length a.base
+
+let alloc2 (#t:Type) (x:t) (n:U32.t)
+  : Steel (array t)
+             emp
+             (fun r -> varray r)
+             (requires fun _ -> True)
+             (ensures fun _ r h1 ->
+               Seq.length r.base == U32.v n /\
+               r.from == 0ul /\
+               Ghost.reveal r.to == n /\
+               asel r h1 == Seq.create (U32.v n) x /\
+               freeable r
+             )
+=
+  let base = valloc n x in
+  let res = {
+    base = base;
+    from = 0ul;
+    to = n;
+  } in
+  intro_varray (Ghost.hide base) res;
+  return res
+
+let alloc x n = alloc2 x n
+
+let index #t r i =
+  let r2 = elim_varray r in
+  let p = unpack_ith r2 i in
+  let gl = gget (varray2 p.ith_lhs) in
+  let gg = gget (vptr p.ith_item) in
+  let gr = gget (varray2 p.ith_rhs) in
+  seq_index_append_cons (U32.v i) (Ghost.reveal gl) (Ghost.reveal gg) (Ghost.reveal gr);
+  (* r2 and p are ghost,
+     so the proper way is to index into base *)
+  seq_index_append_cons (U32.v i) p.ith_lhs p.ith_item p.ith_rhs;
+  let j : nat = U32.v r.from + U32.v i in
+  let pi = Seq.index r.base j in
+  change_equal_slprop (vptr p.ith_item) (vptr pi);
+  let res = read pi in 
+  change_equal_slprop (vptr pi) (vptr p.ith_item);
+  pack_ith p r2;
+  intro_varray r2 r;
+  return res
+
+let upd #t r i x =
+  let r2 = elim_varray r in
+  let p = unpack_ith r2 i in
+  let gl = gget (varray2 p.ith_lhs) in
+  let gg = gget (vptr p.ith_item) in
+  let gr = gget (varray2 p.ith_rhs) in
+  seq_upd_append_cons (U32.v i) x (Ghost.reveal gl) (Ghost.reveal gg) (Ghost.reveal gr);
+  (* r2 and p are ghost,
+     so the proper way is to index into base *)
+  seq_index_append_cons (U32.v i) p.ith_lhs p.ith_item p.ith_rhs;
+  let j : nat = U32.v r.from + U32.v i in
+  let pi = Seq.index r.base j in
+  change_equal_slprop (vptr p.ith_item) (vptr pi);
+  write pi x;
+  change_equal_slprop (vptr pi) (vptr p.ith_item);
+  pack_ith p r2;
+  intro_varray r2 r
+
+(* TODO: properly deallocate instead of just dropping the vprop *)
+let free #t r =
+  reveal_emp ();
+  change_slprop_rel
+    (varray r)
+    (emp)
+    (fun _ _ -> True)
+    (fun m -> intro_emp m)
