ulib/experimental/Steel.Array.fsti
@@ -1,5 +1,5 @@
 (*
-   Copyright 2020 Microsoft Research
+   Copyright 2021 Microsoft Research
 
    Licensed under the Apache License, Version 2.0 (the "License");
    you may not use this file except in compliance with the License.
@@ -20,42 +20,169 @@ open Steel.Effect
 open FStar.Ghost
 module U32 = FStar.UInt32
 
+(* escape hatches to avoid normalization by Steel tactics *)
+
+let pfst
+  (#t1 #t2: Type)
+  (x: (t1 & t2))
+: Pure t1
+  (requires True)
+  (ensures (fun y -> y == fst x))
+= fst x
+
+let psnd
+  (#t1 #t2: Type)
+  (x: (t1 & t2))
+: Pure t2
+  (requires True)
+  (ensures (fun y -> y == snd x))
+= snd x
+
 /// A library for arrays in Steel
 /// TODO: Add fractional permissions to this array library
-
-/// The contents of an array of type [t] is a sequence of values of type [t]
-let contents (t:Type u#0) = FStar.Seq.seq t
-/// Returns the length of the array. Usable for specification and proof purposes,
-/// as modeled by the GTot effect
-let length #t (r:contents t) : GTot nat = Seq.length r
 
 /// Abstract datatype for a Steel array of type [t]
 val array (t:Type u#0) : Type u#0
 
+/// Returns the length of the array. Usable for specification and proof purposes,
+/// as modeled by the GTot effect
+val len (#t: Type) (a: array t) : GTot U32.t
+let length (#t: Type) (a: array t) : GTot nat = U32.v (len a)
+
 /// Separation logic predicate indicating the validity of the array in the current memory
 val is_array (#a:Type0) (r:array a) : slprop u#1
 
-/// Selector for Steel arrays. It returns the contents in memory of the array
-val array_sel (#a:Type0) (r:array a) : selector (contents a) (is_array r)
+/// Selector for Steel arrays. It returns the contents in memory of the array.
+/// The contents of an array of type [t] is a sequence of values of type [t]
+/// whose length is the length of the array
+val array_sel (#a:Type0) (r:array a) : selector (Seq.lseq a (length r)) (is_array r)
 
 /// Combining the elements above to create an array vprop
+
 [@@ __steel_reduce__]
 let varray' #a r : vprop' =
   {hp = is_array r;
-   t = Seq.seq a;
+   t = Seq.lseq a (length r);
    sel = array_sel r}
 
 [@@ __steel_reduce__]
-unfold
 let varray r = VUnit (varray' r)
 
 /// A wrapper to access an array selector more easily.
 /// Ensuring that the corresponding array vprop is in the context is done by
 /// calling a variant of the framing tactic, as defined in Steel.Effect.Common
-[@@ __steel_reduce__]
+/// [@@ __steel_reduce__]
 let asel (#a:Type) (#p:vprop) (r:array a)
   (h:rmem p{FStar.Tactics.with_tactic selector_tactic (can_be_split p (varray r) /\ True)})
+: GTot (Seq.lseq a (length r))
   = h (varray r)
+
+
+/// Splitting an array into subarrays
+
+val adjacent
+  (#t: Type)
+  (r1 r2: array t)
+: Tot prop
+
+val merge
+  (#t: Type)
+  (r1 r2: array t)
+: Ghost (array t)
+  (requires (adjacent r1 r2))
+  (ensures (fun r -> length r == length r1 + length r2))
+
+let merge_into
+  (#t: Type)
+  (r1 r2 r3: array t)
+: Tot prop
+= adjacent r1 r2 /\
+  merge r1 r2 == r3
+
+val merge_assoc
+  (#t: Type)
+  (r1 r2 r3: array t)
+: Lemma
+  (requires (adjacent r1 r2 /\ adjacent r2 r3))
+  (ensures (
+    adjacent r1 r2 /\ adjacent r2 r3 /\
+    begin
+      let r12 = merge r1 r2 in
+      let r23 = merge r2 r3 in
+      adjacent r1 r23 /\ adjacent r12 r3 /\
+      merge r1 r23 == merge r12 r3
+    end
+  ))
+  [SMTPat (merge (merge r1 r2) r3)]
+
+val merge_zero_left
+  (#t: Type)
+  (r1 r2: array t)
+: Lemma
+  (requires (adjacent r1 r2 /\ length r1 == 0))
+  (ensures (
+    merge_into r1 r2 r2
+  ))
+
+val merge_zero_right
+  (#t: Type)
+  (r1 r2: array t)
+: Lemma
+  (requires (adjacent r1 r2 /\ length r2 == 0))
+  (ensures (
+    merge_into r1 r2 r1
+  ))
+
+val gsplit
+  (#t: Type)
+  (r: array t)
+  (i: U32.t)
+: Ghost (array t & array t)
+  (requires (U32.v i <= length r))
+  (ensures (fun (rl, rr) ->
+    merge_into rl rr r /\
+    length rl == U32.v i
+  ))
+
+val gsplit_unique
+  (#t: Type)
+  (r rl rr: array t)
+: Lemma
+  (requires (merge_into rl rr r))
+  (ensures (
+    (rl, rr) == gsplit r (len rl)
+  ))
+
+val split (#t:Type) (a:array t) (i:U32.t)
+  : Steel (array t & array t)
+          (varray a)
+          (fun res -> varray (pfst res) `star` varray (psnd res))
+          (fun _ -> U32.v i <= length a)
+          (fun h res h' ->
+            let s = h (varray a) in
+            let sl = h' (varray (pfst res)) in
+            let sr = h' (varray (psnd res)) in
+            U32.v i <= length a /\
+            res == gsplit a i /\
+            sl == Seq.slice s 0 (U32.v i) /\
+            sr == Seq.slice s (U32.v i) (length a)
+          )
+
+val join (#t:Type) (al ar:array t)
+  : Steel (array t)
+          (varray al `star` varray ar)
+          (fun a -> varray a)
+          (fun _ -> adjacent al ar)
+          (fun h a h' ->
+            let s = h' (varray a) in
+            s == (h (varray al) `Seq.append` h (varray ar)) /\
+            merge_into al ar a
+          )
+
+/// A property telling that an array "is a full allocation unit"
+/// that can be freed all at once (as opposed to a strict subarray of
+/// some other array)
+val freeable (#t: Type) (a: array t) : Tot prop
 
 /// Allocates an array of length n, where all elements of the array initially are [x]
 val alloc (#t:Type) (x:t) (n:U32.t)
@@ -63,7 +190,10 @@ val alloc (#t:Type) (x:t) (n:U32.t)
              emp
              (fun r -> varray r)
              (requires fun _ -> True)
-             (ensures fun _ r h1 -> asel r h1 == Seq.create (U32.v n) x)
+             (ensures fun _ r h1 ->
+               asel r h1 == Seq.create (U32.v n) x /\
+               freeable r
+             )
 
 /// Accesses index [i] in array [r], as long as [i] is in bounds and the array
 /// is currently valid in memory
@@ -71,11 +201,12 @@ val index (#t:Type) (r:array t) (i:U32.t)
   : Steel t
              (varray r)
              (fun _ -> varray r)
-             (requires fun h -> U32.v i < length (asel r h))
+             (requires fun _ -> U32.v i < length r)
              (ensures fun h0 x h1 ->
-               U32.v i < length (asel r h1) /\
-               asel r h0 == asel r h1 /\
-               x == Seq.index (asel r h1) (U32.v i))
+               let s = asel r h1 in
+               U32.v i < length r /\
+               asel r h0 == s /\
+               x == Seq.index s (U32.v i))
 
 /// Updates index [i] in array [r] with value [x], as long as [i]
 /// is in bounds and the array is currently valid in memory
@@ -83,9 +214,9 @@ val upd (#t:Type) (r:array t) (i:U32.t) (x:t)
   : Steel unit
              (varray r)
              (fun _ -> varray r)
-             (requires fun h -> U32.v i < length (asel r h))
+             (requires fun h -> U32.v i < length r)
              (ensures fun h0 _ h1 ->
-               U32.v i < length (asel r h0) /\
+               U32.v i < length r /\
                asel r h1 == Seq.upd (asel r h0) (U32.v i) x)
 
 /// Frees array [r], as long as it initially was a valid array in memory
@@ -93,11 +224,11 @@ val free (#t:Type) (r:array t)
   : Steel unit
              (varray r)
              (fun _ -> emp)
-             (requires fun _ -> True)
+             (requires fun _ -> freeable r)
              (ensures fun _ _ _ -> True)
 
-
-(* AF: Non-selector version of the Array module, currently unused in Steel
+(* AF: Non-selector version of the Array module, with permissions,
+   currently unused in Steel
    TODO: Port this to the selector version
 
 let contents (t:Type u#0) = erased (FStar.Seq.seq t)
