ulib/experimental/Steel.ArrayPtr.fst
@@ -1,0 +1,273 @@
+(*
+   Copyright 2021 Microsoft Research
+
+   Licensed under the Apache License, Version 2.0 (the "License");
+   you may not use this file except in compliance with the License.
+   You may obtain a copy of the License at
+
+       http://www.apache.org/licenses/LICENSE-2.0
+
+   Unless required by applicable law or agreed to in writing, software
+   distributed under the License is distributed on an "AS IS" BASIS,
+   WITHOUT WARRANTIES OR CONDITIONS OF ANY KIND, either express or implied.
+   See the License for the specific language governing permissions and
+   limitations under the License.
+*)
+
+module Steel.ArrayPtr
+open Steel.Reference
+
+(* We could implement this module as a pointer to an array, 
+   but we would like to be as close as possible to C 
+   pointers, i.e. as base+offset.
+ *)
+friend Steel.Array
+module A = Steel.Array
+
+let to_v
+  (#t: Type)
+  (base: A.array1 t)
+  (from: U32.t)
+: Tot Type0
+= (to: U32.t { U32.v from <= U32.v to /\ U32.v to <= Seq.length base })
+
+let to_t
+  (#t: Type)
+  (base: A.array1 t)
+  (from: U32.t)
+: Tot Type0
+= Ghost.erased (to_v base from)
+
+noeq
+type t (a: Type u#0) = {
+  base: A.array1 a;
+  from: U32.t;
+  to: ghost_ref (to_v base from);
+}
+
+let mk_t (#a: Type u#0) (base: A.array1 a) (from: U32.t) (to: ghost_ref (to_v base from)) : Tot (t a) =
+  {
+    base = base;
+    from = from;
+    to = to;
+  }
+
+let array_of
+  (#a: Type)
+  (p: t a)
+  (to: to_t p.base p.from)
+: Tot (A.array a)
+= {
+  A.base = p.base;
+  A.from = p.from;
+  A.to = Ghost.hide (Ghost.reveal to);
+}
+
+let varrayptr0_dep
+  (#a: Type)
+  (p: t a)
+  (to: normal (t_of (ghost_vptr p.to)))
+: Tot vprop
+= A.varray (array_of p to)
+
+let varrayptr0_rewrite
+  (#a: Type)
+  (p: t a)
+  (x: normal (t_of (ghost_vptr p.to `vdep` varrayptr0_dep p)))
+: Tot (v a)
+= let (| to, contents |) = x in
+  {
+    array = array_of p to;
+    contents = contents;
+  }
+
+let varrayptr0
+  (#a: Type)
+  (r: t a)
+: Tot vprop
+= (ghost_vptr r.to `vdep` varrayptr0_dep r) `vrewrite` varrayptr0_rewrite r
+
+let is_arrayptr #a r = hp_of (varrayptr0 r)
+
+let arrayptr_sel #a r = fun h -> sel_of (varrayptr0 r) h
+
+let intro_varrayptr
+  (#opened: _)
+  (#a: Type)
+  (r: t a)
+: SteelGhost unit opened
+    ((ghost_vptr r.to `vdep` varrayptr0_dep r) `vrewrite` varrayptr0_rewrite r)
+    (fun _ -> varrayptr r)
+    (fun _ -> True)
+    (fun h0 _ h1 -> h1 (varrayptr r) == h0 ((ghost_vptr r.to `vdep` varrayptr0_dep r) `vrewrite` varrayptr0_rewrite r))
+=
+  change_slprop_rel
+    ((ghost_vptr r.to `vdep` varrayptr0_dep r) `vrewrite` varrayptr0_rewrite r)
+    (varrayptr r)
+    (fun x y -> x == y)
+    (fun _ -> ())
+
+let elim_varrayptr
+  (#opened: _)
+  (#a: Type)
+  (r: t a)
+: SteelGhost unit opened
+    (varrayptr r)
+    (fun _ -> (ghost_vptr r.to `vdep` varrayptr0_dep r) `vrewrite` varrayptr0_rewrite r)
+    (fun _ -> True)
+    (fun h0 _ h1 -> h0 (varrayptr r) == h1 ((ghost_vptr r.to `vdep` varrayptr0_dep r) `vrewrite` varrayptr0_rewrite r))
+=
+  change_slprop_rel
+    (varrayptr r)
+    ((ghost_vptr r.to `vdep` varrayptr0_dep r) `vrewrite` varrayptr0_rewrite r)
+    (fun x y -> x == y)
+    (fun _ -> ())
+
+#push-options "--z3rlimit 32"
+let join #opened #a al ar =
+  elim_varrayptr al;
+  elim_vrewrite (ghost_vptr al.to `vdep` varrayptr0_dep al) (varrayptr0_rewrite al);
+  let g_al_to = elim_vdep (ghost_vptr al.to) (varrayptr0_dep al) in
+  let al_to = ghost_read al.to in
+  let aal = array_of al al_to in
+  change_equal_slprop
+    (varrayptr0_dep al (Ghost.reveal g_al_to))
+    (A.varray aal);
+  elim_varrayptr ar;
+  elim_vrewrite (ghost_vptr ar.to `vdep` varrayptr0_dep ar) (varrayptr0_rewrite ar);
+  let g_ar_to = elim_vdep (ghost_vptr ar.to) (varrayptr0_dep ar) in
+  let ar_to = ghost_read ar.to in
+  ghost_free ar.to;
+  let aar = array_of ar ar_to in
+  change_equal_slprop
+    (varrayptr0_dep ar (Ghost.reveal g_ar_to))
+    (A.varray aar);
+  let aj = A.gjoin aal aar in
+  let ar_to : U32.t = ar_to in
+  let ar_to : to_t al.base al.from = ar_to in
+  ghost_write al.to ar_to;
+  assert (Ghost.reveal aj == array_of al ar_to);
+  intro_vdep (ghost_vptr al.to) (A.varray aj) (varrayptr0_dep al);
+  intro_vrewrite (ghost_vptr al.to `vdep` varrayptr0_dep al) (varrayptr0_rewrite al);
+  intro_varrayptr al
+#pop-options
+
+let u32_bounded_add
+  (x y: U32.t) (z: Ghost.erased U32.t)
+: Pure U32.t
+  (requires (U32.v x + U32.v y <= U32.v z))
+  (ensures (fun t -> U32.v t == U32.v x + U32.v y))
+=
+  x `U32.add` y
+
+#push-options "--z3rlimit 32"
+#restart-solver
+let split #a x i =
+  elim_varrayptr x;
+  elim_vrewrite (ghost_vptr x.to `vdep` varrayptr0_dep x) (varrayptr0_rewrite x);
+  let x_to_1 : to_t x.base x.from = elim_vdep (ghost_vptr x.to) (varrayptr0_dep x) in
+  let xa = array_of x x_to_1 in
+  change_equal_slprop
+    (varrayptr0_dep x (Ghost.reveal x_to_1))
+    (A.varray xa);
+  let res2 : Ghost.erased (A.array a & A.array a) = A.gsplit0 xa i in
+  reveal_star (A.varray (A.pfst res2)) (A.varray (A.psnd res2));
+  let x_to_2 : Ghost.erased U32.t = Ghost.hide (Ghost.reveal x_to_1) in
+  let j : to_v x.base x.from = u32_bounded_add x.from i x_to_2 in
+  let x_to_3 : to_t x.base j = Ghost.hide (Ghost.reveal x_to_2) in
+  ghost_write x.to j;
+  assert (A.pfst res2 == array_of x j);
+  intro_vdep
+    (ghost_vptr x.to)
+    (A.varray (A.pfst res2))
+    (varrayptr0_dep x);
+  intro_vrewrite (ghost_vptr x.to `vdep` varrayptr0_dep x) (varrayptr0_rewrite x);
+  intro_varrayptr x;
+  let to2 : ghost_ref (to_v x.base j) = ghost_alloc x_to_3 in
+  let res : t a = mk_t x.base j to2 in
+  let x_to_4 : to_t res.base res.from = Ghost.hide (Ghost.reveal x_to_3 <: U32.t) in
+  assert (A.psnd res2 == array_of res x_to_4);
+  change_equal_slprop
+    (ghost_vptr to2)
+    (ghost_vptr res.to);
+  intro_vdep
+    (ghost_vptr res.to)
+    (A.varray (A.psnd res2))
+    (varrayptr0_dep res);
+  intro_vrewrite (ghost_vptr res.to `vdep` varrayptr0_dep res) (varrayptr0_rewrite res);
+  intro_varrayptr res;
+  return res
+#pop-options
+
+let alloc
+  #a x n
+=
+  Seq.slice_length (Seq.create (U32.v n) x);
+  let ar = A.alloc2 x n in
+  let n2 : to_t ar.A.base 0ul = n in
+  let to : ghost_ref (to_v ar.A.base 0ul) = ghost_alloc n2 in
+  let res = {
+    base = ar.A.base;
+    from = 0ul;
+    to = to;
+  } in
+  assert (array_of res n2 == ar);
+  change_equal_slprop
+    (ghost_vptr to)
+    (ghost_vptr res.to);
+  intro_vdep
+    (ghost_vptr res.to)
+    (A.varray ar)
+    (varrayptr0_dep res);
+  intro_vrewrite (ghost_vptr res.to `vdep` varrayptr0_dep res) (varrayptr0_rewrite res);
+  intro_varrayptr res;
+  return res
+
+let index
+  #a r i
+=
+  elim_varrayptr r;
+  elim_vrewrite (ghost_vptr r.to `vdep` varrayptr0_dep r) (varrayptr0_rewrite r);
+  let g = elim_vdep (ghost_vptr r.to) (varrayptr0_dep r) in
+  let to = ghost_read r.to in
+  let ar = array_of r to in
+  change_equal_slprop
+    (varrayptr0_dep r (Ghost.reveal g))
+    (A.varray ar);
+  let res = A.index ar i in
+  intro_vdep
+    (ghost_vptr r.to)
+    (A.varray ar)
+    (varrayptr0_dep r);
+  intro_vrewrite (ghost_vptr r.to `vdep` varrayptr0_dep r) (varrayptr0_rewrite r);
+  intro_varrayptr r;
+  return res
+
+let upd
+  #a r i x
+=
+  elim_varrayptr r;
+  elim_vrewrite (ghost_vptr r.to `vdep` varrayptr0_dep r) (varrayptr0_rewrite r);
+  let to = elim_vdep (ghost_vptr r.to) (varrayptr0_dep r) in
+  let ar = array_of r to in
+  change_equal_slprop
+    (varrayptr0_dep r (Ghost.reveal to))
+    (A.varray ar);
+  A.upd ar i x;
+  intro_vdep
+    (ghost_vptr r.to)
+    (A.varray ar)
+    (varrayptr0_dep r);
+  intro_vrewrite (ghost_vptr r.to `vdep` varrayptr0_dep r) (varrayptr0_rewrite r);
+  intro_varrayptr r
+
+let free #a r =
+  elim_varrayptr r;
+  elim_vrewrite (ghost_vptr r.to `vdep` varrayptr0_dep r) (varrayptr0_rewrite r);
+  let to = elim_vdep (ghost_vptr r.to) (varrayptr0_dep r) in
+  ghost_free r.to;
+  let ar = array_of r to in
+  change_equal_slprop
+    (varrayptr0_dep r to)
+    (A.varray ar);
+  A.free ar
